Fix type spec and proofs for rigid type variables
Unification too permissive: now split into rigid type variables
that cannot be unified, and free type variables which can
Involves changes to typechecker, spec, and proofs
Added test cases for various edge cases

Strata/DL/Imperative/TypeContext.lean
@@ -38,6 +38,7 @@ class TypeContext (P : PureExpr) (Context TypeEnv TypeError : Type) where
   inferType    : Context → TypeEnv → Cmd P → P.Expr → Except TypeError (P.Expr × P.Ty × TypeEnv)
   unifyTypes   : TypeEnv → List (P.Ty × P.Ty) → Except TypeError TypeEnv
   typeErrorFmt : TypeError → Std.Format
+  checkAnnotCompat : Context → TypeEnv → P.Ty → Except TypeError Unit
 
 ---------------------------------------------------------------------
 end -- public section
